Update definitions batch_op_logic and batch_op

dataplane/Examples/Batch/Batch_Op.thy
@@ -8,25 +8,21 @@ imports
 begin
 
 definition batch_op_logic where
-  "batch_op_logic ips ops comb os logic = notifier_op ips ops os 
-   (\<lambda> os compl_caps.
-    let comb_caps = comb compl_caps in
-    if (\<forall> p. comb_caps p = []) then trace (STR ''No capabilities'') {||} else
-    let compl_batches = (\<lambda> p t. map (de1 os o fst) (filter (\<lambda> (d, t'). t' = t \<and> t \<in> set (comb_caps p)) (input os p))) in
-    let ts = (\<lambda> p. remdups (map snd (filter (\<lambda> (d, t). t \<in> set (comb_caps p)) (input os p)))) in
-    let os = os\<lparr> input := (\<lambda> p. filter (\<lambda> (d, t). t \<notin> set (comb_caps p)) (input os p)) \<rparr> in
-    let outs_drops = logic compl_batches ts comb_caps in
-    cimage (\<lambda> (outs, drops). 
-    trace (STR ''outs: '' + show_nat (length outs) + STR '' , drops: '' + show_nat (length drops))
-    (drop_caps (produces os (map (\<lambda> (d, cap). (en2 os d, cap)) outs)) drops)) outs_drops)"
-
+  \<open>batch_op_logic ps f g os caps =
+  (let caps' = g caps in if \<forall>p. p |\<in>| ps \<longrightarrow> caps' p = [] then trace (STR ''No capabilities'') {||} else
+    let batches = (\<lambda>p t. map (de1 os \<circ> fst) (filter (\<lambda>(d, t'). t' = t \<and> t \<in> set (caps' p)) (input os p)));
+        ts = (\<lambda>p. remdups (map snd (filter (\<lambda>(d, t). t \<in> set (caps' p)) (input os p))));
+        os' = os\<lparr>input := (\<lambda>p. filter (\<lambda>(d, t). t \<notin> set (caps' p)) (input os p))\<rparr>;
+        outs_drops = cUnion (cimage (\<lambda>p. {|(concat (map (\<lambda>t. map (\<lambda>x. (x, Cap t p)) (f (batches p t))) (ts p)), map (\<lambda>t. Cap t p) (caps p))|}) ps)
+    in cimage (\<lambda>(outs, drops).
+      trace (STR ''outs: '' + show_nat (length outs) + STR '' , drops: '' + show_nat (length drops))
+      (drop_caps (produces os' (map (\<lambda>(d, cap). (en2 os' d, cap)) outs)) drops)) outs_drops)\<close>
 
 definition batch_op where
-  "batch_op os f = batch_op_logic {|(1 :: 1)|} {|(1 :: 1)|} id os
-   (\<lambda> compl_batches ts caps. {| (concat (map (\<lambda> t. map (\<lambda> x. (x, Cap t 1)) (f (compl_batches 1 t))) (ts 1)), map (\<lambda> t. Cap t 1) (caps 1)) |})"
+  \<open>batch_op ps f g os = notifier_op ps ps os (batch_op_logic ps f g)\<close>
 
 lemma nop_leaf_batch_op:
-  "nop_leaf None (batch_op os f)"
+  "nop_leaf None (batch_op ps f g os)"
   unfolding batch_op_def batch_op_logic_def notifier_op_def
   by (rule nop_leaf_builder_op) simp
 section \<open>The Batch Dataflow Program\<close>
@@ -69,7 +65,7 @@ abbreviation init_operator_state_ty2 where
    \<rparr>"
 
 abbreviation "input_dt ip_state \<equiv> ((Logic (ooo_input_op {|1 :: 1|} ip_state) default_internal_summary) :: ('a, _, (_, 't) shared_state + (1 \<Rightarrow> 't antichain), 'c \<times> 't, 't :: {ccompare,canonically_ordered_monoid_add,ordered_ab_semigroup_monoid_add_imp_le,bot}) dataflow_tree)"
-abbreviation "batch_dt os2 f \<equiv> Logic (batch_op os2 f) default_internal_summary"
+abbreviation "batch_dt os2 f \<equiv> Logic (batch_op {|1 :: 1|} f id os2) default_internal_summary"
 abbreviation "G f ip_state os2 \<equiv>
   (input_dt (ip_state :: (1, 'd1 + 'd2, 'd1, _) input_state) :: (2, _, _, _, _) dataflow_tree)
     \<sqdot>\<^bsub>1\<^esub> batch_dt (os2 :: (1, 'd1 + 'd2, 'd1, 'd2, _) operator_state_ty2) f"
